Try to improve transitions in chapter 4

Listings/SpecCert.v
@@ -258,339 +258,306 @@ Section SpecCert.
       exact Htrans.
   Qed.
 
-  Section Isolation.
-    Inductive software_stack
-    : Type :=
-    | BIOS
-      : software_stack
-    | OS
-      : software_stack
-    | App (n:  nat)
-      : software_stack.
+  Inductive software_stack
+  : Type :=
+  | BIOS
+    : software_stack
+  | OS
+    : software_stack
+  | App (n:  nat)
+    : software_stack.
 
-    Variables (ss_context:  S -> software_stack)
-              (ss_fetched:  S -> label -> (software_stack -> Prop)).
+  Variables (ss_context:  S -> software_stack)
+            (ss_fetched:  S -> label -> (software_stack -> Prop)).
 
-    Inductive stack_ge
-      : software_stack -> software_stack -> Prop :=
-    | stack_ge_refl (x:  software_stack)
-      : stack_ge x x
-    | bios_bottom (x:  software_stack)
-      : stack_ge BIOS x
-    | os_apps (n:  nat)
-      : stack_ge OS (App n).
+  Inductive stack_ge
+    : software_stack -> software_stack -> Prop :=
+  | stack_ge_refl (x:  software_stack)
+    : stack_ge x x
+  | bios_bottom (x:  software_stack)
+    : stack_ge BIOS x
+  | os_apps (n:  nat)
+    : stack_ge OS (App n).
 
-    Require Import Coq.Arith.PeanoNat.
-    Require Import Coq.Logic.Decidable.
-    Require Coq.Logic.Classical_Prop.
+  Require Import Coq.Arith.PeanoNat.
+  Require Import Coq.Logic.Decidable.
+  Require Coq.Logic.Classical_Prop.
 
-    Definition stack_ge_dec
+  Definition stack_ge_decidable
+           (x y:  software_stack)
+    : stack_ge x y \/ ~ stack_ge x y.
+    refine (
+        match x, y with
+        | BIOS, _
+        | OS, OS
+        | OS, App _
+          => _
+        | _, _
+          => _
+        end
+      );
+      try (left; constructor).
+    + right; intros Hge; inversion Hge.
+    + induction y.
+      ++ right; intros Hge; inversion Hge.
+      ++ right; intros Hge; inversion Hge.
+      ++ destruct (Nat.eq_dec n n0); subst.
+         +++ left; constructor.
+         +++ right; intros Hge; inversion Hge.
+             subst.
+             apply n1.
+             reflexivity.
+  Qed.
+
+  Lemma stack_ge_asym
+    : forall (x y:  software_stack),
+      x <> y -> stack_ge x y -> ~ stack_ge y x.
+  Proof.
+    induction x;
+      intros y Hneq Hge Hnge;
+      inversion Hnge;
+      subst;
+      try (apply Hneq; reflexivity);
+      try (inversion Hge).
+  Qed.
+
+  Lemma stack_ge_trans
+    : forall (x y z:  software_stack),
+      stack_ge x y -> stack_ge y z -> stack_ge x z.
+  Proof.
+    induction x;
+      intros y z Hge1 Hge2;
+      inversion Hge1;
+      inversion Hge2;
+      subst;
+      try constructor;
+      try discriminate.
+  Qed.
+
+  Definition tamper_with
+             {m:    model}
+             (tr:   transition m)
              (x y:  software_stack)
-      : { stack_ge x y } + { ~ stack_ge x y }.
-      refine (
-          match x, y with
-          | BIOS, _
-          | OS, OS
-          | OS, App _
-            => _
-          | _, _
-            => _
-          end
-        );
-        try (left; constructor).
-      + right; intros Hge; inversion Hge.
-      + induction y.
-        ++ right; intros Hge; inversion Hge.
-        ++ right; intros Hge; inversion Hge.
-        ++ destruct (Nat.eq_dec n n0); subst.
-           +++ left; constructor.
-           +++ right; intros Hge; inversion Hge.
-               subst.
-               apply n1.
-               reflexivity.
-    Qed.
+    : Prop :=
+    ss_fetched (from [tr]) (labelled [tr]) y
+    /\ ss_context (from [tr]) = y.
 
-    Lemma stack_ge_asym
-      : forall (x y:  software_stack),
-        x <> y -> stack_ge x y -> ~ stack_ge y x.
-    Proof.
-      induction x;
-        intros y Hneq Hge Hnge;
-        inversion Hnge;
-        subst;
-        try (apply Hneq; reflexivity);
-        try (inversion Hge).
-    Qed.
+  Definition isolation_policy
+             {m:   model}
+             (tr:  transition m)
+    : Prop :=
+    forall (x y:  software_stack),
+      tamper_with tr x y
+      -> stack_ge x y.
 
-    Lemma stack_ge_trans
-      : forall (x y z:  software_stack),
-        stack_ge x y -> stack_ge y z -> stack_ge x z.
-    Proof.
-      induction x;
-        intros y z Hge1 Hge2;
-        inversion Hge1;
-        inversion Hge2;
-        subst;
-        try constructor;
-        try discriminate.
-    Qed.
+  Corollary isolation_policy_aux
+            {m:   model}
+            (tr:  transition m)
+    : isolation_policy tr
+      <-> forall (x y:  software_stack),
+        ~ stack_ge x y -> ~ tamper_with tr x y.
+  Proof.
+    split.
+    + intros Hiso x y Hnge Htamper.
+      unfold isolation_policy in Hiso.
+      apply Hiso in Htamper.
+      apply Hnge.
+      exact Htamper.
+    + intros Hc x y.
+      apply contrapositive.
+      ++ apply stack_ge_decidable.
+      ++ intros Hneq.
+         apply Hc.
+         exact Hneq.
+  Qed.
 
-    Definition tamper_with
-               {m:    model}
-               (tr:   transition m)
-               (x y:  software_stack)
-      : Prop :=
-      ss_fetched (from [tr]) (labelled [tr]) y
-      /\ ss_context (from [tr]) = y.
+  Definition is_tcb
+             (U:  software_stack -> Prop)
+             (x:  software_stack)
+    : Prop :=
+    ~ U x /\ forall (u:  software_stack), U u -> stack_ge x u.
 
-    Definition isolation_policy
-               {m:   model}
-               (tr:  transition m)
-      : Prop :=
-      forall (x y:  software_stack),
-        tamper_with tr x y
-        -> stack_ge x y.
+  Definition constrain_to_isolation
+             {m:   model}
+             (U:   software_stack -> Prop)
+             (tr:  transition m)
+    : Prop :=
+    forall (u y:  software_stack),
+      U u
+      -> tamper_with tr u y
+      -> stack_ge u y.
 
-    Ltac not_not_tac Hnnge :=
-      match goal with
-      | [ |- stack_ge ?x ?y ]
-        => assert (Hf:  ~ stack_ge x y) by (intros Hge; inversion Hge);
-           apply Hnnge in Hf;
-           destruct Hf
-      end.
+  Inductive os_only
+    : software_stack -> Prop :=
+  | OS_only
+    : os_only OS.
 
-    Lemma not_not_stack_ge
-      : forall (x y:  software_stack),
-        ~ (~ stack_ge x y) -> stack_ge x y.
-    Proof.
-      induction x; induction y; try (intros Hnnge; constructor);
-        intros Hnnge;
-        try not_not_tac Hnnge.
-      destruct (Nat.eq_dec n n0).
-      + subst.
-        constructor.
-      + assert (Hf:  ~ stack_ge (App n) (App n0)). {
-          intros Hf.
-          inversion Hf.
-          subst.
-          apply n1.
-          reflexivity.
-        }
-        apply Hnnge in Hf.
-        destruct Hf.
-    Qed.
+  Inductive apps_only
+    : software_stack -> Prop :=
+  | Apps_only (n:  nat)
+    : apps_only (App n).
 
-    Corollary isolation_policy_aux
-              {m:   model}
-              (tr:  transition m)
-      : isolation_policy tr
-        <-> forall (x y:  software_stack),
-          ~ stack_ge x y -> ~ tamper_with tr x y.
-    Proof.
+  Definition compatible_hse
+             {m:  model}
+             (hse1 hse2:  HSE m)
+    : Prop :=
+    software hse1 = software hse2
+    /\ forall x H,
+      context hse2 x = eq_rect _ id (context hse1 x) _ H.
+
+  Definition HSE_cap
+             {m:            model}
+             (hse1 hse2:    HSE m)
+             (Hcompatible:  compatible_hse hse1 hse2)
+    : HSE m.
+    refine ({| software := software hse1
+             ; context  := context hse1
+             ; tcb := fun x
+                      => tcb hse1 x \/ tcb hse2 (eq_rect _ id x _ _)
+             ; inv := fun x
+                      => inv hse1 x /\ inv hse2 x
+             ; behaviour := fun x l
+                            => behaviour hse1 x l /\ behaviour hse2 x l
+             |}).
+    + intros tr [Hi1 Hi2] Hsoft.
+      split; apply law_1; [exact Hi1 | idtac | exact Hi2 | idtac];
+         induction tr as [tr Htr]; induction tr as [[h l] h'];
+         induction l; auto;
+         apply Hsoft.
+    + intros tr Htcb.
+      apply Classical_Prop.not_or_and in Htcb.
+      destruct Htcb as [Ht1 Ht2].
+      inversion Hcompatible as [Hsoftware Hcontext].
+      rewrite <- Hcontext in Ht2.
+      apply law_2 in Ht1.
+      apply law_2 in Ht2.
+      induction tr as [tr Htr];
+        induction tr as [[h l] h'];
+        induction l; auto.
+      unfold proj1_sig.
       split.
-      + intros Hiso x y Hnge Htamper.
-        unfold isolation_policy in Hiso.
-        apply Hiso in Htamper.
-        apply Hnge.
-        exact Htamper.
-      + intros Hc x y.
-        apply contrapositive.
-        ++ destruct (stack_ge_dec x y); [left | right]; assumption.
-        ++ intros Hneq.
-           apply Hc.
-           exact Hneq.
-    Qed.
+      ++ apply Ht1.
+      ++ apply Ht2.
+      Unshelve.
+      apply Hcompatible.
+  Defined.
 
-    Definition is_tcb
-               (U:  software_stack -> Prop)
-               (x:  software_stack)
-      : Prop :=
-      ~ U x /\ forall (u:  software_stack), U u -> stack_ge x u.
-
-    Definition constrain_to_isolation
-               {m:   model}
-               (U:   software_stack -> Prop)
-               (tr:  transition m)
-      : Prop :=
-      forall (u y:  software_stack),
-        U u
-        -> tamper_with tr u y
-        -> stack_ge u y.
-
-    Inductive os_only
-      : software_stack -> Prop :=
-    | OS_only
-      : os_only OS.
-
-    Inductive apps_only
-      : software_stack -> Prop :=
-    | Apps_only (n:  nat)
-      : apps_only (App n).
-
-    Require Import Coq.Program.Equality.
-
-    Definition compatible_hse
-               {m:  model}
-               (hse1 hse2:  HSE m)
-      : Prop :=
-      software hse1 = software hse2
-      /\ forall x H,
-        context hse2 x = eq_rect _ id (context hse1 x) _ H.
-
-    Definition HSE_cap
-               {m:            model}
-               (hse1 hse2:    HSE m)
-               (Hcompatible:  compatible_hse hse1 hse2)
-      : HSE m.
-      refine ({| software := software hse1
-               ; context  := context hse1
-               ; tcb := fun x
-                        => tcb hse1 x \/ tcb hse2 (eq_rect _ id x _ _)
-               ; inv := fun x
-                        => inv hse1 x /\ inv hse2 x
-               ; behaviour := fun x l
-                              => behaviour hse1 x l /\ behaviour hse2 x l
-               |}).
-      + intros tr [Hi1 Hi2] Hsoft.
-        split; apply law_1; [exact Hi1 | idtac | exact Hi2 | idtac];
-           induction tr as [tr Htr]; induction tr as [[h l] h'];
-           induction l; auto;
-           apply Hsoft.
-      + intros tr Htcb.
-        apply Classical_Prop.not_or_and in Htcb.
-        destruct Htcb as [Ht1 Ht2].
-        inversion Hcompatible as [Hsoftware Hcontext].
-        rewrite <- Hcontext in Ht2.
-        apply law_2 in Ht1.
-        apply law_2 in Ht2.
-        induction tr as [tr Htr];
-          induction tr as [[h l] h'];
-          induction l; auto.
-        unfold proj1_sig.
-        split.
-        ++ apply Ht1.
-        ++ apply Ht2.
-        Unshelve.
-        apply Hcompatible.
-    Defined.
-
-    Lemma compliant_trace_intersec_sketches
-          (P P' R Q Q':  Prop)
-      : (P /\ P') /\ (R -> Q /\ Q')
-        <-> (P /\ (R -> Q)) /\ (P' /\ (R -> Q')).
-    Proof.
+  Lemma compliant_trace_intersec_sketches
+        (P P' R Q Q':  Prop)
+    : (P /\ P') /\ (R -> Q /\ Q')
+      <-> (P /\ (R -> Q)) /\ (P' /\ (R -> Q')).
+  Proof.
+    split.
+    + intros [[Hp Hp'] Hr].
       split.
-      + intros [[Hp Hp'] Hr].
-        split.
-        ++ split.
-           +++ exact Hp.
-           +++ intros Hr'.
-               apply Hr in Hr'.
-               apply Hr'.
-        ++ split.
-           +++ exact Hp'.
-           +++ intros Hr'.
-               apply Hr in Hr'.
-               apply Hr'.
-      + intros [[Hp Hq] [Hp' Hq']].
-        split.
-        ++ split; assumption.
-        ++ intros Hr.
-           auto.
-    Qed.
-
-    Lemma compliant_trace_intersec_intersec_compliant_trace
-          {m:      model}
-          (hse_1:  HSE m)
-          (hse_2:  HSE m)
-          (Hcomp:  compatible_hse hse_1 hse_2)
-          (rho:    trace m)
-      : compliant_trace (HSE_cap hse_1 hse_2 Hcomp) rho
-        -> compliant_trace hse_1 rho /\ compliant_trace hse_2 rho.
-    Proof.
-      intros Hct.
-      unfold compliant_trace in Hct.
-      unfold HSE_cap in Hct.
-      cbn in Hct.
+      ++ split.
+         +++ exact Hp.
+         +++ intros Hr'.
+             apply Hr in Hr'.
+             apply Hr'.
+      ++ split.
+         +++ exact Hp'.
+         +++ intros Hr'.
+             apply Hr in Hr'.
+             apply Hr'.
+    + intros [[Hp Hq] [Hp' Hq']].
       split.
-      + constructor.
-        ++ apply Hct.
-        ++ intros tr Htr.
-           destruct Hct as [_H H].
-           assert (Hres:  if_software (labelled [tr])
-                                      (fun l : Ls =>
-                                         behaviour hse_1 (from [tr]) l
-                                         /\ behaviour hse_2 (from [tr]) l))
-             by (apply H; exact Htr).
-           induction tr as [tr _H2]; induction tr as [[h l] h'].
-           induction l; auto.
-           cbn in *.
-           apply Hres.
-      + constructor.
-        ++ apply Hct.
-        ++ intros tr Htr.
-           destruct Hct as [_H H].
-           assert (Hres:  if_software (labelled [tr])
-                                      (fun l : Ls =>
-                                         behaviour hse_1 (from [tr]) l
-                                         /\ behaviour hse_2 (from [tr]) l))
-             by (apply H; exact Htr).
-           induction tr as [tr _H2]; induction tr as [[h l] h'].
-           induction l; auto.
-           cbn in *.
-           apply Hres.
-    Qed.
+      ++ split; assumption.
+      ++ intros Hr.
+         auto.
+  Qed.
 
-    Lemma intersec_compliant_trace_compliant_trace_intersec
-          {m:      model}
-          (hse_1:  HSE m)
-          (hse_2:  HSE m)
-          (Hcomp:  compatible_hse hse_1 hse_2)
-          (rho:    trace m)
-      : compliant_trace hse_1 rho /\ compliant_trace hse_2 rho
-        -> compliant_trace (HSE_cap hse_1 hse_2 Hcomp) rho.
-    Proof.
-      intros [H1 H2].
-      constructor.
-      + unfold HSE_cap.
-        cbn.
-        split; [apply H1|apply H2].
-      + intros tr Htrans.
-        assert (Hb1:  if_software (labelled [tr])
-                                  (behaviour hse_1 (from [tr])))
-          by (apply H1; exact Htrans).
-        assert (Hb2:  if_software (labelled [tr])
-                                  (behaviour hse_2 (from [tr])))
-          by (apply H2; exact Htrans).
-        induction tr as [tr _H3]; induction tr as [[h l] h'].
-        induction l; cbn in *; auto.
-    Qed.
+  Lemma compliant_trace_intersec_intersec_compliant_trace
+        {m:      model}
+        (hse_1:  HSE m)
+        (hse_2:  HSE m)
+        (Hcomp:  compatible_hse hse_1 hse_2)
+        (rho:    trace m)
+    : compliant_trace (HSE_cap hse_1 hse_2 Hcomp) rho
+      -> compliant_trace hse_1 rho /\ compliant_trace hse_2 rho.
+  Proof.
+    intros Hct.
+    unfold compliant_trace in Hct.
+    unfold HSE_cap in Hct.
+    cbn in Hct.
+    split.
+    + constructor.
+      ++ apply Hct.
+      ++ intros tr Htr.
+         destruct Hct as [_H H].
+         assert (Hres:  if_software (labelled [tr])
+                                    (fun l : Ls =>
+                                       behaviour hse_1 (from [tr]) l
+                                       /\ behaviour hse_2 (from [tr]) l))
+           by (apply H; exact Htr).
+         induction tr as [tr _H2]; induction tr as [[h l] h'].
+         induction l; auto.
+         cbn in *.
+         apply Hres.
+    + constructor.
+      ++ apply Hct.
+      ++ intros tr Htr.
+         destruct Hct as [_H H].
+         assert (Hres:  if_software (labelled [tr])
+                                    (fun l : Ls =>
+                                       behaviour hse_1 (from [tr]) l
+                                       /\ behaviour hse_2 (from [tr]) l))
+           by (apply H; exact Htr).
+         induction tr as [tr _H2]; induction tr as [[h l] h'].
+         induction l; auto.
+         cbn in *.
+         apply Hres.
+  Qed.
 
-    Theorem constrain_everyone
-            {m:         model}
-            (hse_bios:  HSE m)
-            (hse_os:    HSE m)
-            (Hcomp:     compatible_hse hse_bios hse_os)
-      : correct_hse hse_bios
-                    (safety_property (constrain_to_isolation os_only))
-        -> correct_hse hse_os
-                       (safety_property (constrain_to_isolation apps_only))
-        -> correct_hse (HSE_cap hse_bios hse_os Hcomp)
-                       (safety_property isolation_policy).
-    Proof.
-      intros Hbios Hos rho Hct tr Htrans.
-      apply compliant_trace_intersec_intersec_compliant_trace in Hct.
-      inversion Hct as [Hrb Hro].
-      intros x y Htamper.
-      unfold correct_hse, safety_property, constrain_to_isolation in *.
-      induction x.
-      + constructor.
-      + apply (Hbios rho Hrb tr Htrans).
-        ++ constructor.
-        ++ exact Htamper.
-      + apply (Hos rho Hro tr Htrans).
-        ++ constructor.
-        ++ exact Htamper.
-    Qed.
-  End Isolation.
+  Lemma intersec_compliant_trace_compliant_trace_intersec
+        {m:      model}
+        (hse_1:  HSE m)
+        (hse_2:  HSE m)
+        (Hcomp:  compatible_hse hse_1 hse_2)
+        (rho:    trace m)
+    : compliant_trace hse_1 rho /\ compliant_trace hse_2 rho
+      -> compliant_trace (HSE_cap hse_1 hse_2 Hcomp) rho.
+  Proof.
+    intros [H1 H2].
+    constructor.
+    + unfold HSE_cap.
+      cbn.
+      split; [apply H1|apply H2].
+    + intros tr Htrans.
+      assert (Hb1:  if_software (labelled [tr])
+                                (behaviour hse_1 (from [tr])))
+        by (apply H1; exact Htrans).
+      assert (Hb2:  if_software (labelled [tr])
+                                (behaviour hse_2 (from [tr])))
+        by (apply H2; exact Htrans).
+      induction tr as [tr _H3]; induction tr as [[h l] h'].
+      induction l; cbn in *; auto.
+  Qed.
+
+  Theorem constrain_everyone
+          {m:         model}
+          (hse_bios:  HSE m)
+          (hse_os:    HSE m)
+          (Hcomp:     compatible_hse hse_bios hse_os)
+    : correct_hse hse_bios
+                  (safety_property (constrain_to_isolation os_only))
+      -> correct_hse hse_os
+                     (safety_property (constrain_to_isolation apps_only))
+      -> correct_hse (HSE_cap hse_bios hse_os Hcomp)
+                     (safety_property isolation_policy).
+  Proof.
+    intros Hbios Hos rho Hct tr Htrans.
+    apply compliant_trace_intersec_intersec_compliant_trace in Hct.
+    inversion Hct as [Hrb Hro].
+    intros x y Htamper.
+    unfold correct_hse, safety_property, constrain_to_isolation in *.
+    induction x.
+    + constructor.
+    + apply (Hbios rho Hrb tr Htrans).
+      ++ constructor.
+      ++ exact Htamper.
+    + apply (Hos rho Hro tr Htrans).
+      ++ constructor.
+      ++ exact Htamper.
+  Qed.
 End SpecCert.
